arm/proofs/mlkem_ntt.ml
@@ -421,28 +421,6 @@ let ntt_constants = define
 (* Some convenient proof tools.                                              *)
 (* ------------------------------------------------------------------------- *)
 
-let READ_MEMORY_MERGE_CONV =
-  let baseconv =
-    GEN_REWRITE_CONV I [READ_MEMORY_BYTESIZED_SPLIT] THENC
-    LAND_CONV(LAND_CONV(RAND_CONV(RAND_CONV
-     (TRY_CONV(GEN_REWRITE_CONV I [GSYM WORD_ADD_ASSOC] THENC
-               RAND_CONV WORD_ADD_CONV))))) in
-  let rec conv n tm =
-    if n = 0 then REFL tm else
-    (baseconv THENC BINOP_CONV (conv(n - 1))) tm in
-  conv;;
-
-let READ_MEMORY_SPLIT_CONV =
-  let baseconv =
-    GEN_REWRITE_CONV I [READ_MEMORY_BYTESIZED_UNSPLIT] THENC
-    BINOP_CONV(LAND_CONV(LAND_CONV(RAND_CONV(RAND_CONV
-     (TRY_CONV(GEN_REWRITE_CONV I [GSYM WORD_ADD_ASSOC] THENC
-               RAND_CONV WORD_ADD_CONV)))))) in
-  let rec conv n tm =
-    if n = 0 then REFL tm else
-    (baseconv THENC BINOP_CONV (conv(n - 1))) tm in
-  conv;;
-
 let SIMD_SIMPLIFY_CONV =
   TOP_DEPTH_CONV
    (REWR_CONV WORD_SUBWORD_AND ORELSEC WORD_SIMPLE_SUBWORD_CONV) THENC
@@ -455,16 +433,6 @@ let SIMD_SIMPLIFY_TAC =
    (ASSUME_TAC o
     CONV_RULE(RAND_CONV SIMD_SIMPLIFY_CONV) o
     check (simdable o concl)));;
-
-let MEMORY_128_FROM_16_TAC =
-  let a_tm = `a:int64` and n_tm = `n:num` and i64_ty = `:int64`
-  and pat = `read (memory :> bytes128(word_add a (word n))) s0` in
-  fun v n ->
-    let pat' = subst[mk_var(v,i64_ty),a_tm] pat in
-    let f i =
-      let itm = mk_small_numeral(16*i) in
-      READ_MEMORY_MERGE_CONV 3 (subst[itm,n_tm] pat') in
-    MP_TAC(end_itlist CONJ (map f (0--(n-1))));;
 
 (* ------------------------------------------------------------------------- *)
 (* Correctness proof.                                                        *)
